src/program_proof/mvcc/tuple_read_version.v
@@ -197,15 +197,16 @@ Definition tuple_read tuple tid key val found γ : iProp Σ :=
 Definition per_key_cmt_inv_def key tmods tid m past future γ : iProp Σ :=
   per_key_inv_def γ key tmods tid m past ∗ cmt_inv_def γ tmods future.
 
-Lemma tuple_read_safe tid ts key tmods m past future tuple val found γ :
-  head_read future tid key ->
+Lemma tuple_read_safe (tid : u64) ts key tmods m past future tuple val found γ :
+  let tidN := (int.nat tid) in 
+  head_read future tidN key ->
   ([∗ set] k ∈ keys_all, per_key_inv_def γ k tmods ts m past) -∗
   cmt_inv_def γ tmods future -∗
   tuple_read tuple tid key val found γ ==∗
-  ([∗ set] k ∈ keys_all, per_key_inv_def γ k tmods ts m (past ++ [EvRead tid key])) ∗
+  ([∗ set] k ∈ keys_all, per_key_inv_def γ k tmods ts m (past ++ [EvRead tidN key])) ∗
   cmt_inv_def γ tmods future ∗
   own_tuple tuple key γ ∗
-  ptuple_ptsto γ key (to_dbval found val) (int.nat tid).
+  ptuple_ptsto γ key (to_dbval found val) tidN.
 Admitted.
 
 (*
